Array verifies in Stacked ST effect

examples/low-level/ulib/FStar.StackArray.fst
@@ -1,11 +1,12 @@
 module FStar.StackArray
 
-#set-options "--max_fuel 0 --initial_fuel 0 --initial_ifuel 0 --max_ifuel 0"
+//#set-options "--max_fuel 0 --initial_fuel 0 --initial_ifuel 0 --max_ifuel 0"
+
 open FStar.Seq
 open FStar.StackHeap
 open FStar.SST
 
-(* abstract *) type array (t:Type0) = ref (seq t)
+(* abstract *) type array (t:Type) = ref (seq t)
 
 assume val op_At_Bar: #a:Type -> array a -> array a -> St (array a)
 
@@ -21,13 +22,17 @@ assume val to_seq: #a:Type -> s:array a -> ST (seq a)
   (requires (fun h -> contains h s))
   (ensures  (fun h0 x h1 -> (sel h0 s=x /\ h0==h1)))
 
-assume val create : #a:Type -> n:nat -> init:a -> ST (array a)
+val create : #a:Type -> n:nat -> init:a -> ST (array a)
   (requires (fun h -> True))
   (ensures  (fun h0 x h1 -> (not(contains h0 x)
 		             /\ frameOf x = top_frame_id h1
                              /\ contains h1 x
-                             /\ modifies !{} h0 h1
-                             /\ sel h1 x=Seq.create n init)))
+			     /\ stack h1 = stack h0
+			     /\ modifies_one (top_frame_id h1) h0 h1
+			     /\ modifies_ref (top_frame_id h1) !{asRef x} h0 h1	                    
+			     /\ sel h1 x = Seq.create n init
+			     )))
+let create #a n init = salloc (Seq.create n init)
 
 assume val index : #a:Type -> x:array a -> n:nat -> ST a
   (requires (fun h -> contains h x /\ n < Seq.length (sel h x)))
@@ -77,29 +82,33 @@ val copy_aux:
 			    /\ (ctr <= Seq.length (sel h cpy))
 			    /\ (forall (i:nat). i < ctr ==> Seq.index (sel h s) i = Seq.index (sel h cpy) i)))
 	(ensures (fun h0 u h1 -> (contains h1 s /\ contains h1 cpy /\ s <> cpy )
+			      /\ modifies_one (frameOf cpy) h0 h1
 			      /\ (modifies_ref (frameOf cpy) !{as_ref (refOf cpy)} h0 h1)
-			      /\ (Seq.equal (sel h1 cpy) (sel h1 s))))
+			      /\ (Seq.equal (sel h1 cpy) (sel h1 s))
+			      /\ stack h1 = stack h0))
 let rec copy_aux #a s cpy ctr =
   match length cpy - ctr with
   | 0 -> ()
   | _ -> upd cpy ctr (index s ctr);
 	 copy_aux s cpy (ctr+1)
 
-(*
-
 val copy:
   #a:Type -> s:array a ->
   ST (array a) 
      (requires (fun h -> contains h s
 			 /\ Seq.length (sel h s) > 0))
-     (ensures (fun h0 r h1 -> (modifies !{} h0 h1)
-		                     /\ frameOf r = top_frame_id h1
-				     /\ not(contains h0 r)
-				     /\ (contains h1 r)
-				     /\ (Seq.equal (sel h1 r) (sel h0 s)))) 
+     (ensures (fun h0 r h1 -> modifies_one (top_frame_id h1) h0 h1
+			    /\ modifies_ref (top_frame_id h1) !{asRef s} h0 h1
+	                    /\ frameOf r = top_frame_id h1
+			    /\ not(contains h0 r)
+			    /\ (contains h1 r)
+			    /\ (Seq.equal (sel h1 r) (sel h0 s))))
 let copy #a s =
+  let h0 = get () in
   let cpy = create (length s) (index s 0) in
-  copy_aux #a s cpy 0;
+  let h = get () in
+  copy_aux s cpy 0; 
+  let h1 = get () in
   cpy
 
 val blit_aux:
@@ -114,6 +123,7 @@ val blit_aux:
 		    i < ctr ==> Seq.index (sel h s) (s_idx+i) = Seq.index (sel h t) (t_idx+i))))
      (ensures (fun h0 u h1 ->
 	       (contains h1 s /\ contains h1 t /\ s <> t )
+	       /\ stack h1 = stack h0
 	       /\ (modifies (Set.singleton (frameOf t)) h0 h1)
 	       /\ (modifies_ref (frameOf t) !{asRef t} h0 h1)
 	       /\ (Seq.length (sel h1 s) >= s_idx + len)
@@ -135,11 +145,9 @@ let rec blit_aux #a s s_idx t t_idx len ctr =
 	 cut (Map.equal (heaps h) (heaps (StackHeap.upd h0 t (sel h t)))); 
 	 cut (sel h t = Seq.upd (sel h0 t) (t_idx+ctr) (Seq.index (sel h0 s) (s_idx+ctr))); 
 	 cut (forall (i:nat). i < ctr+1 ==> Seq.index (sel h0 s) (s_idx+i) = Seq.index (sel h t) (t_idx+i));
-//	 cut (sel h s = sel h0 s); 
-	 admit()
-
-//	 blit_aux s s_idx t t_idx len (ctr+1)
-
+	 assert(s <> t);
+	 blit_aux s s_idx t t_idx len (ctr+1)
+	 
 val blit:
   #a:Type -> s:array a -> s_idx:nat -> t:array a -> t_idx:nat -> len:nat ->
   ST unit
@@ -151,11 +159,12 @@ val blit:
 		/\ (Seq.length (sel h t) >= t_idx + len)))
      (ensures (fun h0 u h1 ->
 	       (contains h1 s /\ contains h1 t /\ s <> t )
+	       /\ stack h1 = stack h0
 	       /\ (Seq.length (sel h1 s) >= s_idx + len)
 	       /\ (Seq.length (sel h1 t) >= t_idx + len)
 	       /\ (Seq.length (sel h0 s) = Seq.length (sel h1 s))
 	       /\ (Seq.length (sel h0 t) = Seq.length (sel h1 t))
-	       /\ (modifies (Set.singleton (frameOf t)) h0 h1)
+	       /\ (modifies_one (frameOf t) h0 h1)
 	       /\ (modifies_ref (frameOf t) !{asRef t} h0 h1)
 	       /\ (forall (i:nat).
 		   i < len ==> Seq.index (sel h1 s) (s_idx+i) = Seq.index (sel h1 t) (t_idx+i))
@@ -176,7 +185,9 @@ val sub :
       (contains h1 t)
       /\ (contains h0 s)
       /\ not(contains h0 t)
-      /\ (modifies !{} h0 h1)
+      /\ modifies_one (top_frame_id h1) h0 h1
+      /\ modifies_ref (top_frame_id h1) !{asRef t} h0 h1
+      /\ frameOf t = top_frame_id h1
       /\ (Seq.length (sel h0 s) > 0)
       /\ (idx + len <= Seq.length (sel h0 s))
       /\ (Seq.equal (Seq.slice (sel h0 s) idx (idx+len)) (sel h1 t))))
